[refactor] Locally nameless contexts, plus reorganized soft-type related structures

ST/SoftType.v
@@ -19,463 +19,23 @@ Require Import Program.
 From ST Require Import EVarsScratchwork.
 From ST Require Import Vector.
 From ST Require Export Logic.V Logic.Term.
+From ST Require Export SoftType.Radix SoftType.Attribute SoftType.Adjective SoftType.SoftType SoftType.JudgementType.
+From ST Require Export SoftType.LocalContext SoftType.GlobalContext.
 Import ListNotations.
 Import VectorNotations.
 Open Scope string_scope.
 
-
-(** ** Radix Types
-
-These are "mother types". In full Mizar, this is either a [Mode] or a [Struct] 
-or a set (what we call [Ast]).
-*)
-Inductive Radix : Type :=
-| Ast : Radix
-| Mode : forall (n : nat), name -> Vector.t Term n -> Radix.
-
-Definition radix_is_mode (R : Radix) : Prop :=
-  match R with
-  | Mode _ _ _ => True
-  | _ => False
-  end.
-
-Fixpoint vectors_eqb {A : Type} {n1 n2} (v1 : Vector.t A n1) (v2 : Vector.t A n2) (eq : A -> A -> bool) : bool :=
-match v1, v2 with
-| Vector.nil _, Vector.nil _ => true
-| Vector.cons _ h1 k1 t1,  Vector.cons _ h2 k2 t2 => if andb (eqb k1 k2) (eq h1 h2) then (vectors_eqb t1 t2 eq) else false
-| _, _ => false
-end.
-
-Global Instance EqRadix : Eq Radix := {
-  eqb (R1 R2 : Radix) :=
-  match R1,R2 with
-  | Ast, Ast => true
-  | Mode n1 s1 args1, Mode n2 s2 args2 => if andb (eqb n1 n2) (eqb s1 s2) then
-    vectors_eqb args1 args2 term_eqb
-    else false
-  | _, _ => false
-  end
-}.
-
-Global Instance substRadix : Subst Radix :=
-{
-  subst (x : V) (t : Term) (R : Radix) :=
-  match R with
-  | Ast => R
-  | Mode n s args => Mode n s (Vector.map (fun (arg : Term) => subst x t arg) args)
-  end
-}.
-
-Global Instance liftRadix : Lift Radix :=
-{
-  lift (c d : nat) (R : Radix) :=
-  match R with
-  | Ast => R
-  | Mode n s args => Mode n s (Vector.map (fun (a : Term) => lift c d a) args)
-  end
-}.
-
-Global Instance EnumerateEVarsRadix : EnumerateEVars Radix := {
-list_evars R := match R with
-| Ast => []%list
-| Mode n s args => Vector.fold_left (fun l' => fun (arg : Term) => insert_merge (list_evars arg) l') []%list args
-end
-}.
-
-Theorem list_evars_radix_sorted : forall (R : Radix),
-  sorted (list_evars R).
-Proof.
-  intros.
-  induction R.
-  - simpl; auto. apply sorted_nil.
-  - rename t into args.
-    unfold list_evars; unfold EnumerateEVarsRadix.
-    apply insert_merge_vector_fold_sorted2.
-    apply sorted_nil.
-Qed.
-
-(** ** Attributes
-
-Attributes may be prepended to types, when registered in an existential cluster.
-Otherwise, we can create a formula [Term is Attribute]. 
-*)
-
-Inductive Attribute : Type := 
-| Attr : forall (n : nat), name -> Vector.t Term n -> Attribute.
-
-Global Instance EqAttribute : Eq Attribute := {
-  eqb (A1 A2 : Attribute) :=
-  match A1,A2 with
-  | Attr n1 s1 args1, Attr n2 s2 args2 => if andb (eqb n1 n2) (eqb s1 s2) then
-    vectors_eqb args1 args2 term_eqb
-    else false
-  end
-}.
-
-Global Instance substAttr : Subst Attribute :=
-{
-  subst (x : V) (t : Term) (a : Attribute) :=
-  match a with
-  | Attr n s args => Attr n s (Vector.map (fun (arg : Term) => subst x t arg) args)
-  end
-}.
-
-Global Instance liftAttr : Lift Attribute :=
-{
-  lift (c d : nat) (a : Attribute) :=
-  match a with
-  | Attr n s args => Attr n s (Vector.map (fun (a : Term) => lift c d a) args)
-  end
-}.
-
-Global Instance EnumerateEVarsAttribute : EnumerateEVars Attribute := {
-list_evars attr := match attr with
-| Attr n s args => Vector.fold_left (fun l' => fun (arg : Term) => insert_merge (list_evars arg) l') []%list args
-end
-}.
-
-Theorem list_evars_attribute_sorted : forall (A : Attribute),
-  sorted (list_evars A).
-Proof. intros. destruct A. rename t into args.
-  unfold list_evars; unfold EnumerateEVarsAttribute.
-  apply insert_merge_vector_fold_sorted2.
-  apply sorted_nil.
-Qed.
-
-(** ** Adjectives
-
-An adjective is either a "positive [Attribute]" or a "negative [Attribute]".
-*)
-
-Inductive Adjective : Type :=
-| Pos : Attribute -> Adjective
-| Neg : Attribute -> Adjective.
-
-Global Instance EqAdjective : Eq Adjective := {
-  eqb (A1 A2 : Adjective) :=
-  match A1,A2 with
-  | Pos a1, Pos a2 => eqb a1 a2
-  | Neg a1, Neg a2 => eqb a1 a2
-  | _, _ => false
-  end
-}.
-
-Global Instance substAdj : Subst Adjective := {
-  subst (x : V) (t : Term) (alpha : Adjective) :=
-  match alpha with
-  | Pos a => Pos (subst x t a)
-  | Neg a => Neg (subst x t a)
-  end
-}.
-
-Global Instance liftAdj : Lift Adjective :=
-{
-  lift (c d : nat) (alpha : Adjective) :=
-  match alpha with
-  | Pos a => Pos (lift c d a)
-  | Neg a => Neg (lift c d a)
-  end
-}.
-
-Global Instance EnumerateEVarsAdjective : EnumerateEVars Adjective := {
-list_evars adj := match adj with
-| Pos a => list_evars a
-| Neg a => list_evars a
-end
-}.
-
-Theorem list_evars_adjective_sorted : forall (A : Adjective),
-  sorted (list_evars A).
-Proof. intros. destruct A.
-  - assert(list_evars (Pos a) = list_evars a). { simpl; auto. }
-    rewrite H.
-    apply list_evars_attribute_sorted.
-  - assert(list_evars (Neg a) = list_evars a). { simpl; auto. }
-    rewrite H.
-    apply list_evars_attribute_sorted.
-Qed.
-
-(* ** Soft Types
-
-We can encode a [SoftType] as an ordered pair of a list of [Adjective] and
-a [Radix] type.
-*)
-Definition SoftType : Type := (list Adjective)*Radix.
-Definition Star : SoftType := (List.nil, Ast).
-
-Global Instance EqSoftType : Eq SoftType := {
-  eqb (T1 T2 : SoftType) :=
-  match T1,T2 with
-  | (adjs1, R1), (adjs2, R2) => andb (list_eqb adjs1 adjs2 eqb) (eqb R1 R2)
-  end
-}.
-
-Global Instance substSoftType : Subst SoftType := {
-  subst (x : V) (t : Term) (T : SoftType) :=
-  match T with
-  | (List.nil, R) => (List.nil, subst x t R)
-  | (adjs, R) => (List.map (fun (a : Adjective) => subst x t a) adjs, subst x t R)
-  end
-}.
-
-Global Instance liftSoftType : Lift SoftType :=
-{
-  lift (c d : nat) (T : SoftType) :=
-  match T with
-  | (adjs, R) => (List.map (fun (a : Adjective) => (lift c d a)) adjs, lift c d R)
-  end
-}.
-
-Global Instance EnumerateEVarsSoftType : EnumerateEVars SoftType := {
-list_evars T := match T with
-| (adjectives,T) => List.fold_left (fun l' => fun (adj : Adjective) => insert_merge (list_evars adj) l')
- adjectives (list_evars T)
-end
-}.
-
-Theorem list_evars_soft_type_sorted : forall (T : SoftType),
-  sorted (list_evars T).
-Proof. intros. destruct T.
-  assert (sorted (list_evars r)). { apply list_evars_radix_sorted. }
-  unfold list_evars; unfold EnumerateEVarsSoftType.
-  apply insert_merge_list_fold_sorted2 with (init := list_evars r).
-  assumption.
-Qed.
-
-(** *** Miscellaneous predicates concerning soft types *)
-Definition type_is_named (T : SoftType) (n : name) : Prop :=
-  match T with
-  | (_, Mode k1 s1 args1) => n = s1
-  | _ => False
-  end.
-
-Definition mk_mode {n} (M : name) (args : Vector.t Term n) : SoftType :=
-  (List.nil, (Mode n M args)).
-
-Definition prefix (a : Adjective) (T : SoftType) : SoftType :=
-  match T with
-  | (adjs, R) => if List.existsb (fun (adj : Adjective) => eqb a adj) adjs 
-                 then T else (List.cons a adjs, R)
-  end.
-
-Fixpoint prefix_all (adjs : list Adjective) (T : SoftType) : SoftType :=
-  match adjs with
-  | List.nil => T
-  | List.cons a ad2 => prefix_all ad2 (prefix a T)
-  end.
-
-Definition non (a : Adjective) : Adjective :=
-  match a with
-  | Pos attr => Neg attr
-  | Neg attr => Pos attr
-  end.
-
-(** ** Judgement Types *)
-
-Inductive JudgementType :=
-| CorrectContext : JudgementType
-| Esti : Term -> SoftType -> JudgementType
-| Subtype : SoftType -> SoftType -> JudgementType
-| Inhabited : SoftType -> JudgementType
-| HasAttribute : Attribute -> SoftType -> JudgementType.
-
-Global Instance substJudgementType : Subst JudgementType := {
-  subst (x : V) (t : Term) (J : JudgementType) :=
-  match J with
-  | CorrectContext => J
-  | Esti tm Tp => Esti (subst x t tm) (subst x t Tp)
-  | Subtype T1 T2 => Subtype (subst x t T1) (subst x t T2)
-  | Inhabited T => Inhabited (subst x t T)
-  | HasAttribute a T => HasAttribute (subst x t a) (subst x t T)
-  end
-}.
-
-Global Instance liftJudgementType : Lift JudgementType := {
-  lift (c d : nat) (J : JudgementType) :=
-  match J with
-  | CorrectContext => J
-  | Esti tm Tp => Esti (lift c d tm) (lift c d Tp)
-  | Subtype T1 T2 => Subtype (lift c d T1) (lift c d T2)
-  | Inhabited T => Inhabited (lift c d T)
-  | HasAttribute a T => HasAttribute (lift c d a) (lift c d T)
-  end
-}.
-
-Global Instance EnumerateEVarsJudgementType : EnumerateEVars JudgementType := {
-list_evars Judg := match Judg with
-| CorrectContext => []%list
-| Esti t T => insert_merge (list_evars t) (list_evars T)
-| Subtype T1 T2 => insert_merge (list_evars T1) (list_evars T2)
-| Inhabited T => list_evars T
-| HasAttribute a T => insert_merge (list_evars a) (list_evars T)
-end
-}.
-
-Theorem list_evars_judgement_type_sorted : forall (j : JudgementType),
-  sorted (list_evars j).
-Proof.
-  intros. induction j.
-  - unfold list_evars; unfold EnumerateEVarsJudgementType. apply sorted_nil.
-  - unfold list_evars; unfold EnumerateEVarsJudgementType.
-    assert (sorted (list_evars s)). { apply list_evars_soft_type_sorted. }
-    apply insert_merge_sorted2. assumption.
-  - unfold list_evars; unfold EnumerateEVarsJudgementType.
-    assert (sorted (list_evars s0)). { apply list_evars_soft_type_sorted. }
-    apply insert_merge_sorted2. assumption.
-  - unfold list_evars; unfold EnumerateEVarsJudgementType.
-    assert (sorted (list_evars s)). { apply list_evars_soft_type_sorted. }
-    assumption.
-  - unfold list_evars; unfold EnumerateEVarsJudgementType.
-    assert (sorted (list_evars s)). { apply list_evars_soft_type_sorted. }
-    apply insert_merge_sorted2. assumption.
-Qed.
-(** ** Local Contexts
-
-A local context is just a finite list of [Decl] (declaration of variables and
-their types). We will turn this into arguments for a [Term] (or [Attribute], 
-or...), so we have a [local_vars] helper function to accomodate this.
-
-
-TODO: I think this is not quite right. Using locally nameless terms, a 
-declaration simplifies to just a [SoftType]. Then a [LocalContext] is just
-a list of [Decl].
-
-TODO 2: Think hard about whether lifting is necessary for local contexts.
-*)
-Definition Decl : Type := V*SoftType.
-Definition LocalContext := list Decl.
-
-(**
-Given a [LocalContext], we can turn it into a vector of variables, to be used as
-the arguments for a [Term], [Attribute], or [SoftType] (or whatever).
-*)
-Fixpoint local_vars (lc : LocalContext) : Vector.t Term (List.length lc) :=
-  match lc with
-  | List.cons (x,_) tl => (Var x)::(local_vars tl)
-  | List.nil => []
-  end.
-
-Definition evars_local_declaration (d : Decl) :=
-  match d with
-  | (_, T) => (list_evars T)
-  end.
-
-Global Instance EnumerateEVarsLocalContext : EnumerateEVars LocalContext := {
-list_evars lc := List.fold_left (fun l' => fun (d : Decl) => 
-  insert_merge (evars_local_declaration d) l')
- lc []%list
-}.
-
-Theorem list_evars_local_context_sorted : forall (lc : LocalContext),
-  sorted (list_evars lc).
-Proof. intros.
-  unfold list_evars; unfold EnumerateEVarsLocalContext.
-  apply insert_merge_list_fold_sorted. apply sorted_nil.
-Qed.
-
-(* Helper function to turn a [nat] into a [string]. *)
-Fixpoint string_of_nat_aux (time n : nat) (acc : string) : string :=
-  let d := match n mod 10 with
-           | 0 => "0" | 1 => "1" | 2 => "2" | 3 => "3" | 4 => "4" | 5 => "5"
-           | 6 => "6" | 7 => "7" | 8 => "8" | _ => "9"
-           end in
-  let acc' := d ++ acc in
-  match time with
-    | 0 => acc'
-    | S time' =>
-      match n / 10 with
-        | 0 => acc'
-        | n' => string_of_nat_aux time' n' acc'
-      end
-  end.
-
-Definition string_of_nat (n : nat) : string :=
-  string_of_nat_aux n n "".
-
-(** Given a [LocalContext] and a [Term], we can redefine it using the local
-variables from our [LocalContext]. *)
-Definition fun_with_locals (t : Term) (lc : LocalContext) : Term :=
-  match t with
-  | Fun f args => Fun f (local_vars lc)
-  | EConst _ => t
-  | Var var => match var with
-               | FVar x => Fun x (local_vars lc)
-               | BVar n => Fun ("BoundVar_" ++ string_of_nat n) (local_vars lc)
-               end
-  end.
-  
-Definition mode_with_locals (R : Radix) (lc : LocalContext) : Radix :=
-  match R with
-  | Ast => Ast
-  | Mode n nm args => Mode (List.length lc) nm (local_vars lc)
-  end.
-
-Fixpoint lc_is_subcontext (subcontext lc : LocalContext) : Prop :=
-  match subcontext with
-  | List.cons (x,T) subcontext' => List.In (x,T) lc /\ lc_is_subcontext subcontext' lc
-  | List.nil => True
-  end.
-
-(** ** Global Contexts
-
-We now can track definitions of terms, types, etc., using a [GlobalContext].
-This is encoded as just a list of [JudgementType] and the relevant local 
-variables as found in a [LocalContext].
-*)
-Definition GlobalContext := list (LocalContext * JudgementType).
-
-
-Definition list_evars_gc_def (d : LocalContext * JudgementType) :=
-match d with
-  | (lc, T) => insert_merge (list_evars lc) (list_evars T)
-  end.
-
-Global Instance EnumerateEVarsGlobalContext : EnumerateEVars GlobalContext := {
-list_evars gc := List.fold_left (fun l' => fun d => 
-  insert_merge (list_evars_gc_def d)  l')
- gc []%list
-}.
-
-Theorem list_evars_global_context_sorted : forall (gc : GlobalContext),
-  sorted (list_evars gc).
-Proof.
-  intros.
-  unfold list_evars; unfold EnumerateEVarsGlobalContext.
-  apply insert_merge_list_fold_sorted. apply sorted_nil.
-Qed.
-
-
-(** Judgements of the form [t : T] are where we define new constant terms. *)
-Fixpoint gc_defines_term (gc : GlobalContext) (n : name) : Prop :=
-  match gc with
-  | List.cons (lc, Esti (Fun nm _) T) tl => (n = nm) \/ gc_defines_term tl n
-  | _ => False
-  end.
-
-Fixpoint gc_defines_type (gc : GlobalContext) (n : name) : Prop :=
-  match gc with
-  | List.cons (lc, Subtype T1 T2) tl => (type_is_named T1 n) \/ (type_is_named T2 n) \/ (gc_defines_type  tl n)
-  | List.cons (lc, Inhabited T) tl =>(type_is_named T n) \/ (gc_defines_type  tl n)
-  | _ => False
-  end.
-
-Fixpoint gc_defines_attr (gc : GlobalContext) (n : name) : Prop :=
-  match gc with
-  | List.cons (lc, HasAttribute (Attr _ a args) T) tl => (a = n) \/ (gc_defines_attr tl n)
-  | _ => False
-  end.
-
-Fixpoint gc_contains (Γ : GlobalContext) (def : (LocalContext * JudgementType)) : Prop :=
-  match Γ,def with
-  | List.cons (lc, J') Γ', (subcontext, J) => ((lc_is_subcontext subcontext lc) /\ J = J') \/ gc_contains Γ' def
-  | List.nil, _ => False
-  end.
 
 (** * Inference Rules for Soft Types
 
 We can now code up the inference rules for Wiedijk's soft type system inductively. 
 *)
 Definition Judgement : Type := GlobalContext * LocalContext * JudgementType.
+
+Definition Judgement_body (j : Judgement) :=
+match j with
+| (_,_, body) => body
+end.
 
 Global Instance EnumerateEVarsJudgement : EnumerateEVars Judgement := {
 list_evars j := match j with
@@ -495,21 +55,30 @@ Proof. intros. destruct j.
   apply insert_merge_sorted2; assumption.
 Qed.
 
+Check subst.
 
 Definition push {A : Type} (a : A) (l : list A) : list A :=
   List.app l (List.cons a List.nil).
-
+Close Scope string_scope.
+Import ListNotations.
+  
 Notation "gc ;; lc |- j" := (gc, lc, j) (at level 80).
+Import ListNotations.
+Open Scope list_scope.
 Inductive well_typed : Judgement -> Prop :=
-| wt_empty_context : well_typed (List.nil ;; List.nil |- CorrectContext)
-| wt_var : forall (Γ : GlobalContext) (Δ : LocalContext) (x : V) (T : SoftType) (J : JudgementType),
+| wt_empty_context : well_typed ([] ;; [] |- CorrectContext)
+| wt_var : forall (Γ : GlobalContext) (Δ : LocalContext) (T : SoftType) (J : JudgementType),
   well_typed (Γ ;; Δ |- Inhabited T) ->
-  well_typed (Γ ;; (push (x,T) Δ) |- CorrectContext)
+  well_typed (Γ ;; (push T Δ) |- CorrectContext)
 (* TODO: substitution rule for a vector of declarations *)
-| wt_subst : forall (Γ : GlobalContext) (Δ : LocalContext) (x : V) (t : Term) (T : SoftType) (J : JudgementType),
-  gc_contains Γ ((List.cons (x,T) List.nil), J) ->
+| wt_subst : forall (Γ : GlobalContext) (Δ Δ' : LocalContext) (t : Term) (T : SoftType) (J : JudgementType),
+  gc_contains Γ ((List.cons T Δ), J) ->
   well_typed (Γ ;; Δ |- Esti t T) ->
-  well_typed (Γ ;; Δ |- (subst x t J))
+  well_typed (Γ ;; Δ |- (subst (BVar 0) t J))
+(* XXX Wiedijk combines this [wt_assume] rule with [wt_subst] in a single step, I decompose them into two. *)
+| wt_assume : forall (Γ : GlobalContext) (Δ : LocalContext) (J : JudgementType),
+  gc_contains Γ (Δ, J) ->
+  well_typed (Γ ;; Δ |- J)
 (* TODO: inhabited types produce new local variables *)
 | wt_subtype_star_star : forall (Γ : GlobalContext) (Δ : LocalContext),
   well_typed (Γ ;; Δ |- CorrectContext) ->
@@ -554,22 +123,22 @@ Inductive well_typed : Judgement -> Prop :=
 | wt_functor_def : forall (Γ : GlobalContext) (Δ : LocalContext) (T : SoftType) (f : name),
   not (gc_defines_term Γ f) ->
   well_typed (Γ ;; Δ |- Inhabited T) ->
-  well_typed ((List.app Γ (List.cons (Δ, (Esti (Fun f (local_vars Δ)) T)) List.nil)) ;; List.nil |- CorrectContext)
+  well_typed (Γ ++ [(Δ, (Esti (Fun f (local_vars Δ)) T))] ;; [] |- CorrectContext)
 | wt_mode_def : forall (Γ : GlobalContext) (Δ : LocalContext) (T : SoftType) (M : name), 
   not (gc_defines_type Γ M) ->
   well_typed (Γ ;; Δ |- Inhabited T) ->  
-  well_typed ((List.app Γ 
-              (List.cons (Δ, (Subtype (mk_mode M (local_vars Δ)) T))
-                (List.cons (Δ, (Inhabited (mk_mode M (local_vars Δ)))) List.nil))) ;; List.nil |- CorrectContext)
+  well_typed (Γ ++
+              [(Δ, (Subtype (mk_mode M (local_vars Δ)) T)) ;
+                (Δ, (Inhabited (mk_mode M (local_vars Δ))))] ;; [] |- CorrectContext)
 | wt_attr_def : forall (Γ : GlobalContext) (Δ : LocalContext) (T : SoftType) (alpha : name), 
   not (gc_defines_attr Γ alpha) ->
   well_typed (Γ ;; Δ |- Inhabited T) ->
-  well_typed (List.app Γ (List.cons (Δ, HasAttribute (Attr (List.length Δ) alpha (local_vars Δ)) T) List.nil) ;; List.nil |- CorrectContext)
+  well_typed (Γ ++ [(Δ, HasAttribute (Attr (List.length Δ) alpha (local_vars Δ)) T)] ;; List.nil |- CorrectContext)
   (* Rules governing clusters *)
 | wt_cluster_exist : forall (Γ : GlobalContext) (Δ : LocalContext) (T : SoftType) (a : Adjective), 
   well_typed (Γ ;; Δ |- Subtype (prefix a T) T) ->
   well_typed (Γ ;; Δ |- Inhabited T) ->
-  well_typed (List.app Γ (List.cons (Δ, (Inhabited (prefix a T))) List.nil) ;; List.nil |- CorrectContext)
+  well_typed (Γ ++ [(Δ, (Inhabited (prefix a T)))] ;; [] |- CorrectContext)
 | wt_cluster_cond : forall (Γ : GlobalContext) (Δ : LocalContext) (T : SoftType) (a1 a2 : list Adjective), 
   well_typed (Γ ;; Δ |- Subtype (prefix_all a1 T) T) ->
   well_typed (Γ ;; Δ |- Subtype (prefix_all a2 T) T) ->
@@ -577,17 +146,18 @@ Inductive well_typed : Judgement -> Prop :=
 | wt_cluster_fun : forall (Γ : GlobalContext) (Δ : LocalContext) (t : Term) (T : SoftType) (a : Adjective), 
   well_typed (Γ ;; Δ |- Esti t T) ->
   well_typed (Γ ;; Δ |- Subtype (prefix a T) T) ->
-  well_typed (List.app Γ (List.cons (Δ, (Esti t (prefix a T))) List.nil) ;; List.nil |- CorrectContext)
+  well_typed (Γ ++ [(Δ, (Esti t (prefix a T)))] ;; [] |- CorrectContext)
   (* Rules governing redefinitions *)
 | wt_redef_fun : forall (Γ : GlobalContext) (Δ₁ Δ₂ : LocalContext) (t : Term) (T1 T2 T3 : SoftType), 
   term_is_fun t ->
   well_typed (Γ ;; Δ₂ |- Inhabited T2) ->
   well_typed (Γ ;; Δ₂ |- Subtype T2 T3) ->
-  well_typed (Γ ;; (List.app Δ₁ Δ₂) |- Esti (fun_with_locals t Δ₂) T3) ->
-  well_typed ((List.app Γ (List.cons ((List.app Δ₁ Δ₂), (Esti (fun_with_locals t Δ₂) T3)) List.nil)) ;; List.nil |- CorrectContext)
+  well_typed (Γ ;; (Δ₁ ++ Δ₂) |- Esti (fun_with_locals t Δ₂) T3) ->
+  well_typed (Γ ++ [((Δ₁ ++ Δ₂), (Esti (fun_with_locals t Δ₂) T3))] ;; List.nil |- CorrectContext)
 | wt_redef_mode : forall (Γ : GlobalContext) (Δ₁ Δ₂ : LocalContext) (M : Radix) (T1 T2 T3 : SoftType), 
   radix_is_mode M ->
   well_typed (Γ ;; Δ₂ |- Inhabited T2) ->
   well_typed (Γ ;; Δ₂ |- Subtype T2 T3) ->
-  well_typed (Γ ;; (List.app Δ₁ Δ₂) |- Subtype (List.nil, (mode_with_locals M Δ₂)) T3) ->
-  well_typed ((List.app Γ (List.cons ((List.app Δ₁ Δ₂), (Subtype (List.nil, (mode_with_locals M Δ₂)) T3)) List.nil)) ;; List.nil |- CorrectContext).
+  well_typed (Γ ;; (Δ₁ ++ Δ₂) |- Subtype ([], (mode_with_locals M Δ₂)) T3) ->
+  well_typed (Γ ++ [((Δ₁ ++ Δ₂), (Subtype ([], (mode_with_locals M Δ₂)) T3))] ;; [] |- CorrectContext).
+
