ST/SoftType/Adjective.v
@@ -1,0 +1,77 @@
+Require Import String.
+Require Import Lia.
+Require Import List.
+Require Import Nat.
+Require Import Coq.Vectors.Vector.
+Require Import Coq.Vectors.VectorEq.
+Require Import Coq.Arith.Bool_nat.
+Require Export Coq.Arith.Compare_dec.
+Require Import Coq.Arith.EqNat.
+Require Import Coq.Arith.PeanoNat.
+Require Import Coq.Arith.Peano_dec.
+Require Import Coq.Bool.Bool.
+Require Import Coq.Logic.Classical_Prop.
+Require Import Coq.Logic.Eqdep_dec.
+Require Import Coq.Logic.FunctionalExtensionality.
+Require Export RelationClasses.
+Require Export Morphisms.
+Require Import Program.
+From ST Require Import EVarsScratchwork.
+From ST Require Import Vector.
+From ST Require Export Logic.V Logic.Term SoftType.Attribute.
+Import ListNotations.
+Import VectorNotations.
+Open Scope string_scope.
+
+(** ** Adjectives
+
+An adjective is either a "positive [Attribute]" or a "negative [Attribute]".
+*)
+
+Inductive Adjective : Type :=
+| Pos : Attribute -> Adjective
+| Neg : Attribute -> Adjective.
+
+Global Instance EqAdjective : Eq Adjective := {
+  eqb (A1 A2 : Adjective) :=
+  match A1,A2 with
+  | Pos a1, Pos a2 => eqb a1 a2
+  | Neg a1, Neg a2 => eqb a1 a2
+  | _, _ => false
+  end
+}.
+
+Global Instance substAdj : Subst Adjective := {
+  subst (x : V) (t : Term) (alpha : Adjective) :=
+  match alpha with
+  | Pos a => Pos (subst x t a)
+  | Neg a => Neg (subst x t a)
+  end
+}.
+
+Global Instance liftAdj : Lift Adjective :=
+{
+  lift (c d : nat) (alpha : Adjective) :=
+  match alpha with
+  | Pos a => Pos (lift c d a)
+  | Neg a => Neg (lift c d a)
+  end
+}.
+
+Global Instance EnumerateEVarsAdjective : EnumerateEVars Adjective := {
+list_evars adj := match adj with
+| Pos a => list_evars a
+| Neg a => list_evars a
+end
+}.
+
+Theorem list_evars_adjective_sorted : forall (A : Adjective),
+  sorted (list_evars A).
+Proof. intros. destruct A.
+  - assert(list_evars (Pos a) = list_evars a). { simpl; auto. }
+    rewrite H.
+    apply list_evars_attribute_sorted.
+  - assert(list_evars (Neg a) = list_evars a). { simpl; auto. }
+    rewrite H.
+    apply list_evars_attribute_sorted.
+Qed.
