ST/SoftType/Attribute.v
@@ -1,0 +1,72 @@
+Require Import String.
+Require Import Lia.
+Require Import List.
+Require Import Nat.
+Require Import Coq.Vectors.Vector.
+Require Import Coq.Vectors.VectorEq.
+Require Import Coq.Arith.Bool_nat.
+Require Export Coq.Arith.Compare_dec.
+Require Import Coq.Arith.EqNat.
+Require Import Coq.Arith.PeanoNat.
+Require Import Coq.Arith.Peano_dec.
+Require Import Coq.Bool.Bool.
+Require Import Coq.Logic.Classical_Prop.
+Require Import Coq.Logic.Eqdep_dec.
+Require Import Coq.Logic.FunctionalExtensionality.
+Require Export RelationClasses.
+Require Export Morphisms.
+Require Import Program.
+From ST Require Import EVarsScratchwork.
+From ST Require Import Vector.
+From ST Require Export Logic.V Logic.Term.
+From ST Require Export SoftType.Radix.
+Import ListNotations.
+Import VectorNotations.
+Open Scope string_scope.
+(** ** Attributes
+
+Attributes may be prepended to types, when registered in an existential cluster.
+Otherwise, we can create a formula [Term is Attribute]. 
+*)
+
+Inductive Attribute : Type := 
+| Attr : forall (n : nat), name -> Vector.t Term n -> Attribute.
+
+Global Instance EqAttribute : Eq Attribute := {
+  eqb (A1 A2 : Attribute) :=
+  match A1,A2 with
+  | Attr n1 s1 args1, Attr n2 s2 args2 => if andb (eqb n1 n2) (eqb s1 s2) then
+    vectors_eqb args1 args2 term_eqb
+    else false
+  end
+}.
+
+Global Instance substAttr : Subst Attribute :=
+{
+  subst (x : V) (t : Term) (a : Attribute) :=
+  match a with
+  | Attr n s args => Attr n s (Vector.map (fun (arg : Term) => subst x t arg) args)
+  end
+}.
+
+Global Instance liftAttr : Lift Attribute :=
+{
+  lift (c d : nat) (a : Attribute) :=
+  match a with
+  | Attr n s args => Attr n s (Vector.map (fun (a : Term) => lift c d a) args)
+  end
+}.
+
+Global Instance EnumerateEVarsAttribute : EnumerateEVars Attribute := {
+list_evars attr := match attr with
+| Attr n s args => Vector.fold_left (fun l' => fun (arg : Term) => insert_merge (list_evars arg) l') []%list args
+end
+}.
+
+Theorem list_evars_attribute_sorted : forall (A : Attribute),
+  sorted (list_evars A).
+Proof. intros. destruct A. rename t into args.
+  unfold list_evars; unfold EnumerateEVarsAttribute.
+  apply insert_merge_vector_fold_sorted2.
+  apply sorted_nil.
+Qed.
