ST/SoftType/GlobalContext.v
@@ -1,0 +1,83 @@
+Require Import String.
+Require Import Lia.
+Require Import List.
+Require Import Nat.
+Require Import Coq.Vectors.Vector.
+Require Import Coq.Vectors.VectorEq.
+Require Import Coq.Arith.Bool_nat.
+Require Export Coq.Arith.Compare_dec.
+Require Import Coq.Arith.EqNat.
+Require Import Coq.Arith.PeanoNat.
+Require Import Coq.Arith.Peano_dec.
+Require Import Coq.Bool.Bool.
+Require Import Coq.Logic.Classical_Prop.
+Require Import Coq.Logic.Eqdep_dec.
+Require Import Coq.Logic.FunctionalExtensionality.
+Require Export RelationClasses.
+Require Export Morphisms.
+Require Import Program.
+From ST Require Import EVarsScratchwork.
+From ST Require Import Vector.
+From ST Require Export Logic.V Logic.Term.
+From ST Require Export SoftType.Radix SoftType.Attribute SoftType.Adjective SoftType.SoftType SoftType.JudgementType.
+From ST Require Export SoftType.LocalContext.
+Import ListNotations.
+Import VectorNotations.
+Open Scope string_scope.
+
+
+
+(** ** Global Contexts
+
+We now can track definitions of terms, types, etc., using a [GlobalContext].
+This is encoded as just a list of [JudgementType] and the relevant local 
+variables as found in a [LocalContext].
+*)
+Definition GlobalContext := list (LocalContext * JudgementType).
+
+
+Definition list_evars_gc_def (d : LocalContext * JudgementType) :=
+match d with
+  | (lc, T) => insert_merge (list_evars lc) (list_evars T)
+  end.
+
+Global Instance EnumerateEVarsGlobalContext : EnumerateEVars GlobalContext := {
+list_evars gc := List.fold_left (fun l' => fun d => 
+  insert_merge (list_evars_gc_def d)  l')
+ gc []%list
+}.
+
+Theorem list_evars_global_context_sorted : forall (gc : GlobalContext),
+  sorted (list_evars gc).
+Proof.
+  intros.
+  unfold list_evars; unfold EnumerateEVarsGlobalContext.
+  apply insert_merge_list_fold_sorted. apply sorted_nil.
+Qed.
+
+
+(** Judgements of the form [t : T] are where we define new constant terms. *)
+Fixpoint gc_defines_term (gc : GlobalContext) (n : name) : Prop :=
+  match gc with
+  | List.cons (lc, Esti (Fun nm _) T) tl => (n = nm) \/ gc_defines_term tl n
+  | _ => False
+  end.
+
+Fixpoint gc_defines_type (gc : GlobalContext) (n : name) : Prop :=
+  match gc with
+  | List.cons (lc, Subtype T1 T2) tl => (type_is_named T1 n) \/ (type_is_named T2 n) \/ (gc_defines_type  tl n)
+  | List.cons (lc, Inhabited T) tl =>(type_is_named T n) \/ (gc_defines_type  tl n)
+  | _ => False
+  end.
+
+Fixpoint gc_defines_attr (gc : GlobalContext) (n : name) : Prop :=
+  match gc with
+  | List.cons (lc, HasAttribute (Attr _ a args) T) tl => (a = n) \/ (gc_defines_attr tl n)
+  | _ => False
+  end.
+
+Fixpoint gc_contains (Γ : GlobalContext) (def : (LocalContext * JudgementType)) : Prop :=
+  match Γ,def with
+  | List.cons (lc, J') Γ', (subcontext, J) => ((lc_is_subcontext subcontext lc) /\ J = J') \/ gc_contains Γ' def
+  | List.nil, _ => False
+  end.
