ST/SoftType/JudgementType.v
@@ -1,0 +1,87 @@
+Require Import String.
+Require Import Lia.
+Require Import List.
+Require Import Nat.
+Require Import Coq.Vectors.Vector.
+Require Import Coq.Vectors.VectorEq.
+Require Import Coq.Arith.Bool_nat.
+Require Export Coq.Arith.Compare_dec.
+Require Import Coq.Arith.EqNat.
+Require Import Coq.Arith.PeanoNat.
+Require Import Coq.Arith.Peano_dec.
+Require Import Coq.Bool.Bool.
+Require Import Coq.Logic.Classical_Prop.
+Require Import Coq.Logic.Eqdep_dec.
+Require Import Coq.Logic.FunctionalExtensionality.
+Require Export RelationClasses.
+Require Export Morphisms.
+Require Import Program.
+From ST Require Import EVarsScratchwork.
+From ST Require Import Vector.
+From ST Require Export Logic.V Logic.Term.
+From ST Require Export SoftType.Radix SoftType.Attribute SoftType.Adjective SoftType.SoftType.
+Import ListNotations.
+Import VectorNotations.
+Open Scope string_scope.
+
+
+
+(** ** Judgement Types *)
+
+Inductive JudgementType :=
+| CorrectContext : JudgementType
+| Esti : Term -> SoftType -> JudgementType
+| Subtype : SoftType -> SoftType -> JudgementType
+| Inhabited : SoftType -> JudgementType
+| HasAttribute : Attribute -> SoftType -> JudgementType.
+
+Global Instance substJudgementType : Subst JudgementType := {
+  subst (x : V) (t : Term) (J : JudgementType) :=
+  match J with
+  | CorrectContext => J
+  | Esti tm Tp => Esti (subst x t tm) (subst x t Tp)
+  | Subtype T1 T2 => Subtype (subst x t T1) (subst x t T2)
+  | Inhabited T => Inhabited (subst x t T)
+  | HasAttribute a T => HasAttribute (subst x t a) (subst x t T)
+  end
+}.
+
+Global Instance liftJudgementType : Lift JudgementType := {
+  lift (c d : nat) (J : JudgementType) :=
+  match J with
+  | CorrectContext => J
+  | Esti tm Tp => Esti (lift c d tm) (lift c d Tp)
+  | Subtype T1 T2 => Subtype (lift c d T1) (lift c d T2)
+  | Inhabited T => Inhabited (lift c d T)
+  | HasAttribute a T => HasAttribute (lift c d a) (lift c d T)
+  end
+}.
+
+Global Instance EnumerateEVarsJudgementType : EnumerateEVars JudgementType := {
+list_evars Judg := match Judg with
+| CorrectContext => []%list
+| Esti t T => insert_merge (list_evars t) (list_evars T)
+| Subtype T1 T2 => insert_merge (list_evars T1) (list_evars T2)
+| Inhabited T => list_evars T
+| HasAttribute a T => insert_merge (list_evars a) (list_evars T)
+end
+}.
+
+Theorem list_evars_judgement_type_sorted : forall (j : JudgementType),
+  sorted (list_evars j).
+Proof.
+  intros. induction j.
+  - unfold list_evars; unfold EnumerateEVarsJudgementType. apply sorted_nil.
+  - unfold list_evars; unfold EnumerateEVarsJudgementType.
+    assert (sorted (list_evars s)). { apply list_evars_soft_type_sorted. }
+    apply insert_merge_sorted2. assumption.
+  - unfold list_evars; unfold EnumerateEVarsJudgementType.
+    assert (sorted (list_evars s0)). { apply list_evars_soft_type_sorted. }
+    apply insert_merge_sorted2. assumption.
+  - unfold list_evars; unfold EnumerateEVarsJudgementType.
+    assert (sorted (list_evars s)). { apply list_evars_soft_type_sorted. }
+    assumption.
+  - unfold list_evars; unfold EnumerateEVarsJudgementType.
+    assert (sorted (list_evars s)). { apply list_evars_soft_type_sorted. }
+    apply insert_merge_sorted2. assumption.
+Qed.
