ST/SoftType/LocalContext.v
@@ -1,0 +1,117 @@
+Require Import String.
+Require Import Lia.
+Require Import List.
+Require Import Nat.
+Require Import Coq.Vectors.Vector.
+Require Import Coq.Vectors.VectorEq.
+Require Import Coq.Arith.Bool_nat.
+Require Export Coq.Arith.Compare_dec.
+Require Import Coq.Arith.EqNat.
+Require Import Coq.Arith.PeanoNat.
+Require Import Coq.Arith.Peano_dec.
+Require Import Coq.Bool.Bool.
+Require Import Coq.Logic.Classical_Prop.
+Require Import Coq.Logic.Eqdep_dec.
+Require Import Coq.Logic.FunctionalExtensionality.
+Require Export RelationClasses.
+Require Export Morphisms.
+Require Import Program.
+From ST Require Import EVarsScratchwork.
+From ST Require Import Vector.
+From ST Require Export Logic.V Logic.Term.
+From ST Require Export SoftType.Radix SoftType.Attribute SoftType.Adjective SoftType.SoftType.
+Import ListNotations.
+Import VectorNotations.
+Open Scope string_scope.
+
+(** ** Local Contexts
+
+A local context is just a finite list of [Decl] (declaration of variables and
+their types). We will turn this into arguments for a [Term] (or [Attribute], 
+or...), so we have a [local_vars] helper function to accomodate this.
+
+
+TODO: I think this is not quite right. Using locally nameless terms, a 
+declaration simplifies to just a [SoftType]. Then a [LocalContext] is just
+a list of [Decl].
+
+TODO 2: Think hard about whether lifting is necessary for local contexts.
+*)
+Definition Decl : Type := SoftType.
+Definition LocalContext := list SoftType.
+
+(**
+Given a [LocalContext], we can turn it into a vector of variables, to be used as
+the arguments for a [Term], [Attribute], or [SoftType] (or whatever).
+*)
+
+Definition local_vars (lc : LocalContext) : Vector.t Term (List.length lc) :=
+  Vector.map (fun (n : nat) => Var (BVar n))
+  (rev_nat_range_vector (length lc)).
+
+Example local_vars_3 :
+  (local_vars [Star; Star; Star]%list) = [Var (BVar 2); Var (BVar 1); Var (BVar 0)].
+Proof.
+  simpl; auto.
+Qed.
+
+Definition evars_local_declaration (d : Decl) :=
+  match d with
+  | T => (list_evars T)
+  end.
+
+Global Instance EnumerateEVarsLocalContext : EnumerateEVars LocalContext := {
+list_evars lc := List.fold_left (fun l' => fun (d : Decl) => 
+  insert_merge (evars_local_declaration d) l')
+ lc []%list
+}.
+
+Theorem list_evars_local_context_sorted : forall (lc : LocalContext),
+  sorted (list_evars lc).
+Proof. intros.
+  unfold list_evars; unfold EnumerateEVarsLocalContext.
+  apply insert_merge_list_fold_sorted. apply sorted_nil.
+Qed.
+
+(* Helper function to turn a [nat] into a [string]. *)
+Fixpoint string_of_nat_aux (time n : nat) (acc : string) : string :=
+  let d := match n mod 10 with
+           | 0 => "0" | 1 => "1" | 2 => "2" | 3 => "3" | 4 => "4" | 5 => "5"
+           | 6 => "6" | 7 => "7" | 8 => "8" | _ => "9"
+           end in
+  let acc' := d ++ acc in
+  match time with
+    | 0 => acc'
+    | S time' =>
+      match n / 10 with
+        | 0 => acc'
+        | n' => string_of_nat_aux time' n' acc'
+      end
+  end.
+
+Definition string_of_nat (n : nat) : string :=
+  string_of_nat_aux n n "".
+
+(** Given a [LocalContext] and a [Term], we can redefine it using the local
+variables from our [LocalContext]. *)
+Definition fun_with_locals (t : Term) (lc : LocalContext) : Term :=
+  match t with
+  | Fun f args => Fun f (local_vars lc)
+  | EConst _ => t
+  | Var var => match var with
+               | FVar x => Fun x (local_vars lc)
+               | BVar n => Fun ("BoundVar_" ++ string_of_nat n) (local_vars lc)
+               end
+  end.
+  
+Definition mode_with_locals (R : Radix) (lc : LocalContext) : Radix :=
+  match R with
+  | Ast => Ast
+  | Mode n nm args => Mode (List.length lc) nm (local_vars lc)
+  end.
+
+Fixpoint lc_is_subcontext (subcontext lc : LocalContext) : Prop :=
+  match subcontext with
+  | List.cons (x,T) subcontext' => List.In (x,T) lc /\ lc_is_subcontext subcontext' lc
+  | List.nil => True
+  end.
