ST/SoftType/Radix.v
@@ -1,0 +1,93 @@
+Require Import String.
+Require Import Lia.
+Require Import List.
+Require Import Nat.
+Require Import Coq.Vectors.Vector.
+Require Import Coq.Vectors.VectorEq.
+Require Import Coq.Arith.Bool_nat.
+Require Export Coq.Arith.Compare_dec.
+Require Import Coq.Arith.EqNat.
+Require Import Coq.Arith.PeanoNat.
+Require Import Coq.Arith.Peano_dec.
+Require Import Coq.Bool.Bool.
+Require Import Coq.Logic.Classical_Prop.
+Require Import Coq.Logic.Eqdep_dec.
+Require Import Coq.Logic.FunctionalExtensionality.
+Require Export RelationClasses.
+Require Export Morphisms.
+Require Import Program.
+From ST Require Import EVarsScratchwork.
+From ST Require Import Vector.
+From ST Require Export Logic.V Logic.Term.
+Import ListNotations.
+Import VectorNotations.
+Open Scope string_scope.
+(** ** Radix Types
+
+These are "mother types". In full Mizar, this is either a [Mode] or a [Struct] 
+or a set (what we call [Ast]).
+*)
+Inductive Radix : Type :=
+| Ast : Radix
+| Mode : forall (n : nat), name -> Vector.t Term n -> Radix.
+
+Definition radix_is_mode (R : Radix) : Prop :=
+  match R with
+  | Mode _ _ _ => True
+  | _ => False
+  end.
+
+Fixpoint vectors_eqb {A : Type} {n1 n2} (v1 : Vector.t A n1) (v2 : Vector.t A n2) (eq : A -> A -> bool) : bool :=
+match v1, v2 with
+| Vector.nil _, Vector.nil _ => true
+| Vector.cons _ h1 k1 t1,  Vector.cons _ h2 k2 t2 => if andb (eqb k1 k2) (eq h1 h2) then (vectors_eqb t1 t2 eq) else false
+| _, _ => false
+end.
+
+Global Instance EqRadix : Eq Radix := {
+  eqb (R1 R2 : Radix) :=
+  match R1,R2 with
+  | Ast, Ast => true
+  | Mode n1 s1 args1, Mode n2 s2 args2 => if andb (eqb n1 n2) (eqb s1 s2) then
+    vectors_eqb args1 args2 term_eqb
+    else false
+  | _, _ => false
+  end
+}.
+
+Global Instance substRadix : Subst Radix :=
+{
+  subst (x : V) (t : Term) (R : Radix) :=
+  match R with
+  | Ast => R
+  | Mode n s args => Mode n s (Vector.map (fun (arg : Term) => subst x t arg) args)
+  end
+}.
+
+Global Instance liftRadix : Lift Radix :=
+{
+  lift (c d : nat) (R : Radix) :=
+  match R with
+  | Ast => R
+  | Mode n s args => Mode n s (Vector.map (fun (a : Term) => lift c d a) args)
+  end
+}.
+
+Global Instance EnumerateEVarsRadix : EnumerateEVars Radix := {
+list_evars R := match R with
+| Ast => []%list
+| Mode n s args => Vector.fold_left (fun l' => fun (arg : Term) => insert_merge (list_evars arg) l') []%list args
+end
+}.
+
+Theorem list_evars_radix_sorted : forall (R : Radix),
+  sorted (list_evars R).
+Proof.
+  intros.
+  induction R.
+  - simpl; auto. apply sorted_nil.
+  - rename t into args.
+    unfold list_evars; unfold EnumerateEVarsRadix.
+    apply insert_merge_vector_fold_sorted2.
+    apply sorted_nil.
+Qed.
