ST/SoftType/SoftType.v
@@ -1,0 +1,99 @@
+Require Import String.
+Require Import Lia.
+Require Import List.
+Require Import Nat.
+Require Import Coq.Vectors.Vector.
+Require Import Coq.Vectors.VectorEq.
+Require Import Coq.Arith.Bool_nat.
+Require Export Coq.Arith.Compare_dec.
+Require Import Coq.Arith.EqNat.
+Require Import Coq.Arith.PeanoNat.
+Require Import Coq.Arith.Peano_dec.
+Require Import Coq.Bool.Bool.
+Require Import Coq.Logic.Classical_Prop.
+Require Import Coq.Logic.Eqdep_dec.
+Require Import Coq.Logic.FunctionalExtensionality.
+Require Export RelationClasses.
+Require Export Morphisms.
+Require Import Program.
+From ST Require Import EVarsScratchwork.
+From ST Require Import Vector.
+From ST Require Export Logic.V Logic.Term.
+From ST Require Export SoftType.Radix SoftType.Adjective.
+Import ListNotations.
+Import VectorNotations.
+Open Scope string_scope.
+(* ** Soft Types
+
+We can encode a [SoftType] as an ordered pair of a list of [Adjective] and
+a [Radix] type.
+*)
+Definition SoftType : Type := (list Adjective)*Radix.
+Definition Star : SoftType := (List.nil, Ast).
+
+Global Instance EqSoftType : Eq SoftType := {
+  eqb (T1 T2 : SoftType) :=
+  match T1,T2 with
+  | (adjs1, R1), (adjs2, R2) => andb (list_eqb adjs1 adjs2 eqb) (eqb R1 R2)
+  end
+}.
+
+Global Instance substSoftType : Subst SoftType := {
+  subst (x : V) (t : Term) (T : SoftType) :=
+  match T with
+  | (List.nil, R) => (List.nil, subst x t R)
+  | (adjs, R) => (List.map (fun (a : Adjective) => subst x t a) adjs, subst x t R)
+  end
+}.
+
+Global Instance liftSoftType : Lift SoftType :=
+{
+  lift (c d : nat) (T : SoftType) :=
+  match T with
+  | (adjs, R) => (List.map (fun (a : Adjective) => (lift c d a)) adjs, lift c d R)
+  end
+}.
+
+Global Instance EnumerateEVarsSoftType : EnumerateEVars SoftType := {
+list_evars T := match T with
+| (adjectives,T) => List.fold_left (fun l' => fun (adj : Adjective) => insert_merge (list_evars adj) l')
+ adjectives (list_evars T)
+end
+}.
+
+Theorem list_evars_soft_type_sorted : forall (T : SoftType),
+  sorted (list_evars T).
+Proof. intros. destruct T.
+  assert (sorted (list_evars r)). { apply list_evars_radix_sorted. }
+  unfold list_evars; unfold EnumerateEVarsSoftType.
+  apply insert_merge_list_fold_sorted2 with (init := list_evars r).
+  assumption.
+Qed.
+
+(** *** Miscellaneous predicates concerning soft types *)
+Definition type_is_named (T : SoftType) (n : name) : Prop :=
+  match T with
+  | (_, Mode k1 s1 args1) => n = s1
+  | _ => False
+  end.
+
+Definition mk_mode {n} (M : name) (args : Vector.t Term n) : SoftType :=
+  (List.nil, (Mode n M args)).
+
+Definition prefix (a : Adjective) (T : SoftType) : SoftType :=
+  match T with
+  | (adjs, R) => if List.existsb (fun (adj : Adjective) => eqb a adj) adjs 
+                 then T else (List.cons a adjs, R)
+  end.
+
+Fixpoint prefix_all (adjs : list Adjective) (T : SoftType) : SoftType :=
+  match adjs with
+  | List.nil => T
+  | List.cons a ad2 => prefix_all ad2 (prefix a T)
+  end.
+
+Definition non (a : Adjective) : Adjective :=
+  match a with
+  | Pos attr => Neg attr
+  | Neg attr => Pos attr
+  end.
